truesat_src/solver/solver.dfy
@@ -26,9 +26,9 @@ class SATSolver {
     requires formula.getLiteralValue(formula.truthAssignment[..], literal) == -1;
 
     modifies formula.truthAssignment, formula.traceVariable, formula.traceValue,
-             formula.traceDLStart, formula.traceDLEnd, formula`decisionLevel,
-             formula`assignmentsTrace, formula.trueLiteralsCount,
-             formula.falseLiteralsCount;
+            formula.traceDLStart, formula.traceDLEnd, formula`decisionLevel,
+            formula`assignmentsTrace, formula.trueLiteralsCount,
+            formula.falseLiteralsCount;
 
     ensures formula.valid();
     ensures !formula.hasEmptyClause();
@@ -45,6 +45,7 @@ class SATSolver {
     ensures result.SAT? ==> (
       var (variable, val) := formula.convertLVtoVI(literal, value);
       formula.isSatisfiableExtend(formula.truthAssignment[..][variable as int := val]));
+    ensures result.SAT? ==> formula.isSatisfiableTruthAssignment(old(formula.truthAssignment[..]), result.tau)
 
     ensures result.UNSAT? ==> (
       var (variable, val) := formula.convertLVtoVI(literal, value);
@@ -93,6 +94,7 @@ class SATSolver {
 
     ensures result.SAT? ==> formula.validValuesTruthAssignment(result.tau);
     ensures result.SAT? ==> formula.isSatisfiableExtend(formula.truthAssignment[..]);
+    ensures result.SAT? ==> formula.isSatisfiableTruthAssignment(old(formula.truthAssignment[..]), result.tau)
     ensures result.UNSAT? ==>
       !formula.isSatisfiableExtend(formula.truthAssignment[..]);
     ensures formula.countUnsetVariables(formula.truthAssignment[..]) ==
@@ -109,6 +111,7 @@ class SATSolver {
     var isEmpty : bool := formula.getIsEmpty();
     if (isEmpty) {
       formula.isEmpty_sastisfied();
+      // assert formula.isSatisfiableExtend(formula.truthAssignment[..]);
       result := SAT(formula.truthAssignment[..]);
       assert formula.validValuesTruthAssignment(result.tau);
       return result;
@@ -138,22 +141,313 @@ class SATSolver {
 
   /** in a way it is weird that solve does not know in any way about the
   level0unitPropagation. **/
-  method start() returns (result : SAT_UNSAT)
+  method start() returns (result : SAT_UNSAT) // tau may be arbitrary truth assignment
     requires formula.valid();
     requires formula.decisionLevel == -1;
 
     modifies formula.truthAssignment, formula.traceVariable, formula.traceValue,
-             formula.traceDLStart, formula.traceDLEnd, formula`decisionLevel,
-             formula`assignmentsTrace, formula.trueLiteralsCount,
-             formula.falseLiteralsCount;
+            formula.traceDLStart, formula.traceDLEnd, formula`decisionLevel,
+            formula`assignmentsTrace, formula.trueLiteralsCount,
+            formula.falseLiteralsCount;
 
+    ensures formula.valid();
+    ensures result.SAT? ==> formula.validValuesTruthAssignment(result.tau);
+    ensures result.SAT? ==> formula.isSatisfiableExtend(old(formula.truthAssignment[..]));
+    // this is the added postcondition
+    ensures result.SAT? ==> formula.isSatisfiableTruthAssignment(old(formula.truthAssignment[..]), result.tau)
+    ensures result.UNSAT? ==>
+      !formula.isSatisfiableExtend(old(formula.truthAssignment[..]));
+  {
+    formula.level0UnitPropagation();
+    result := solve();
+  }
+  
+
+  method start_counterexample_new() returns (result : SAT_UNSAT) // tau may be arbitrary truth assignment
+    // specification of input
+    requires formula.variablesCount == 2
+    requires formula.clauses == [[1]]
+    requires formula.decisionLevel == -1
+    requires formula.valid()
+    // export output
+    ensures result == SAT([-1,-1])
+    // preconditions
+    ensures old(formula.valid())
+    ensures old(formula.decisionLevel) == -1
+    // modifies
+    modifies formula.truthAssignment, formula.traceVariable, formula.traceValue,
+            formula.traceDLStart, formula.traceDLEnd, formula`decisionLevel,
+            formula`assignmentsTrace, formula.trueLiteralsCount,
+            formula.falseLiteralsCount;
+    // postconditions
     ensures formula.valid();
     ensures result.SAT? ==> formula.validValuesTruthAssignment(result.tau);
     ensures result.SAT? ==> formula.isSatisfiableExtend(old(formula.truthAssignment[..]));
     ensures result.UNSAT? ==>
       !formula.isSatisfiableExtend(old(formula.truthAssignment[..]));
   {
+    result := SAT([-1,-1]);
+    assert formula.validValuesTruthAssignment([1,1]);
+    assert formula.isTauComplete([1,1]);
+    assert formula.isExtendingTau([-1,-1], [1,1]);
+    assert formula.getLiteralValue([1,1], 1) == 1;
+    assert 1 in formula.clauses[0];
+
+    assert formula.isSatisfied([1,1]);
+
+    assert formula.validVariablesCount();
+    assert formula.validClauses();
+    assert formula.validValuesTruthAssignment(formula.truthAssignment[..]);
+  }
+
+  lemma start_counterexample_non_executable_style(f:Formula, f':Formula, result:SAT_UNSAT)
+    // specification of input
+    requires f.variablesCount == 2
+    requires f.clauses == [[1]]
+    requires f.clausesCount == 1
+    requires f.clauseLength.Length == 1
+    requires f.clauseLength[0] == 1
+    requires f.truthAssignment.Length == 2
+    requires f.truthAssignment[0] == -1
+    requires f.truthAssignment[1] == -1
+    requires f.trueLiteralsCount.Length == 1
+    requires f.trueLiteralsCount[0] == 0
+    requires f.falseLiteralsCount.Length == 1
+    requires f.falseLiteralsCount[0] == 0
+    requires f.positiveLiteralsToClauses.Length == 2
+    requires f.negativeLiteralsToClauses.Length == 2
+    requires f.positiveLiteralsToClauses[0] == [0]
+    requires f.positiveLiteralsToClauses[1] == []
+    requires f.negativeLiteralsToClauses[0] == []
+    requires f.negativeLiteralsToClauses[1] == []
+    requires f.decisionLevel == -1
+    requires f.traceVariable.Length == 2
+    requires f.traceVariable[0] == f.traceVariable[1] == 0
+    requires f.traceValue.Length == 2
+    requires f.traceValue[0] == f.traceValue[1] == false
+    requires f.traceDLStart.Length == 2
+    requires f.traceDLStart[0] == f.traceDLStart[1] == 0
+    requires f.traceDLEnd.Length == 2
+    requires f.traceDLEnd[0] == f.traceDLEnd[1] == 0
+    requires f.assignmentsTrace == {}
+    // specification of new f'
+    requires f'.variablesCount == 2
+    requires f'.clauses == [[1]]
+    requires f'.clausesCount == 1
+    requires f'.clauseLength.Length == 1
+    requires f'.clauseLength[0] == 1
+    requires f'.truthAssignment.Length == 2
+    requires f'.truthAssignment[0] == -1
+    requires f'.truthAssignment[1] == -1
+    requires f'.trueLiteralsCount.Length == 1
+    requires f'.trueLiteralsCount[0] == 0
+    requires f'.falseLiteralsCount.Length == 1
+    requires f'.falseLiteralsCount[0] == 0
+    requires f'.positiveLiteralsToClauses.Length == 2
+    requires f'.negativeLiteralsToClauses.Length == 2
+    requires f'.positiveLiteralsToClauses[0] == [0]
+    requires f'.positiveLiteralsToClauses[1] == []
+    requires f'.negativeLiteralsToClauses[0] == []
+    requires f'.negativeLiteralsToClauses[1] == []
+    requires f'.decisionLevel == -1
+    requires f'.traceVariable.Length == 2
+    requires f'.traceVariable[0] == f'.traceVariable[1] == 0
+    requires f'.traceValue.Length == 2
+    requires f'.traceValue[0] == f'.traceValue[1] == false
+    requires f'.traceDLStart.Length == 2
+    requires f'.traceDLStart[0] == f'.traceDLStart[1] == 0
+    requires f'.traceDLEnd.Length == 2
+    requires f'.traceDLEnd[0] == f.traceDLEnd[1] == 0
+    requires f'.assignmentsTrace == {}
+    // references for f
+    requires (f.truthAssignment != f.trueLiteralsCount) &&
+    (f.truthAssignment != f.falseLiteralsCount) &&
+    (f.truthAssignment != f.clauseLength) &&
+    (f.truthAssignment != f.traceVariable) &&
+    (f.truthAssignment != f.traceDLStart) &&
+    (f.truthAssignment != f.traceDLEnd) &&
+    (f.trueLiteralsCount != f.falseLiteralsCount) &&
+    (f.trueLiteralsCount != f.clauseLength) &&
+    (f.trueLiteralsCount != f.traceVariable) &&
+    (f.trueLiteralsCount != f.traceDLStart) &&
+    (f.trueLiteralsCount != f.traceDLEnd) &&
+    (f.falseLiteralsCount != f.clauseLength) &&
+    (f.falseLiteralsCount != f.traceVariable) &&
+    (f.falseLiteralsCount != f.traceDLStart) &&
+    (f.falseLiteralsCount != f.traceDLEnd) &&
+    (f.clauseLength != f.traceVariable) &&
+    (f.clauseLength != f.traceDLStart) &&
+    (f.clauseLength != f.traceDLEnd) &&
+    (f.positiveLiteralsToClauses != f.negativeLiteralsToClauses) &&
+    (f.traceVariable != f.traceDLStart) &&
+    (f.traceVariable != f.traceDLEnd) &&
+    (f.traceDLStart != f.traceDLEnd)
+    // references for f'
+    requires (f.truthAssignment != f'.trueLiteralsCount) &&
+    (f'.truthAssignment != f'.falseLiteralsCount) &&
+    (f'.truthAssignment != f'.clauseLength) &&
+    (f'.truthAssignment != f'.traceVariable) &&
+    (f'.truthAssignment != f'.traceDLStart) &&
+    (f'.truthAssignment != f'.traceDLEnd) &&
+    (f'.trueLiteralsCount != f'.falseLiteralsCount) &&
+    (f'.trueLiteralsCount != f'.clauseLength) &&
+    (f'.trueLiteralsCount != f'.traceVariable) &&
+    (f'.trueLiteralsCount != f'.traceDLStart) &&
+    (f'.trueLiteralsCount != f'.traceDLEnd) &&
+    (f'.falseLiteralsCount != f'.clauseLength) &&
+    (f'.falseLiteralsCount != f'.traceVariable) &&
+    (f'.falseLiteralsCount != f'.traceDLStart) &&
+    (f'.falseLiteralsCount != f'.traceDLEnd) &&
+    (f'.clauseLength != f'.traceVariable) &&
+    (f'.clauseLength != f'.traceDLStart) &&
+    (f'.clauseLength != f'.traceDLEnd) &&
+    (f'.positiveLiteralsToClauses != f'.negativeLiteralsToClauses) &&
+    (f'.traceVariable != f'.traceDLStart) &&
+    (f'.traceVariable != f'.traceDLEnd) &&
+    (f'.traceDLStart != f'.traceDLEnd)
+    // reference between f and f'
+    requires f.truthAssignment == f'.truthAssignment
+    requires f.traceVariable == f'.traceVariable
+    requires f.traceValue == f'.traceValue
+    requires f.traceDLStart == f'.traceDLStart
+    requires f.traceDLEnd == f'.traceDLEnd
+    requires f.trueLiteralsCount == f'.trueLiteralsCount
+    requires f.falseLiteralsCount == f'.falseLiteralsCount
+    // specification of output
+    requires result.SAT?
+    requires result.tau == [-1,-1]
+    // preconditions
+    ensures f.valid();
+    ensures f.decisionLevel == -1;
+    // modifies
+    ensures f'.variablesCount == f.variablesCount
+    ensures f'.clauses == f.clauses
+    ensures f'.clausesCount == f.clausesCount
+    ensures f'.clauseLength.Length == f.clauseLength.Length
+    ensures forall i | 0 <= i < f.clauseLength.Length :: f.clauseLength[i] == f'.clauseLength[i]
+    ensures f'.positiveLiteralsToClauses.Length == f.positiveLiteralsToClauses.Length
+    ensures f'.negativeLiteralsToClauses.Length == f.negativeLiteralsToClauses.Length
+    ensures f.truthAssignment == f'.truthAssignment
+    ensures f.traceVariable == f'.traceVariable
+    ensures f.traceValue == f'.traceValue
+    ensures f.traceDLStart == f'.traceDLStart
+    ensures f.traceDLEnd == f'.traceDLEnd
+    ensures f.trueLiteralsCount == f'.trueLiteralsCount
+    ensures f.falseLiteralsCount == f'.falseLiteralsCount
+    // postconditions
+    ensures f'.valid()
+    ensures result.SAT? ==> f'.validValuesTruthAssignment(result.tau);
+    ensures result.SAT? ==> f'.isSatisfiableExtend(f.truthAssignment[..]);
+    ensures result.UNSAT? ==>
+      !f'.isSatisfiableExtend(f.truthAssignment[..])
+    {
+        // f
+        assert f.validValuesTruthAssignment([1,1]);
+        assert f.isTauComplete([1,1]);
+        assert f.isExtendingTau([-1,-1], [1,1]);
+        assert f.getLiteralValue([1,1], 1) == 1;
+        assert 1 in f.clauses[0];
+
+        assert f.isSatisfied([1,1]);
+
+        assert f.validVariablesCount();
+        assert f.validClauses();
+        assert f.validValuesTruthAssignment(f.truthAssignment[..]);
+
+        // f'
+        assert f'.validValuesTruthAssignment([1,1]);
+        assert f'.isTauComplete([1,1]);
+        assert f'.isExtendingTau([-1,-1], [1,1]);
+        assert f'.getLiteralValue([1,1], 1) == 1;
+        assert 1 in f.clauses[0];
+
+        assert f'.isSatisfied([1,1]);
+
+        assert f'.validVariablesCount();
+        assert f'.validClauses();
+        assert f'.validValuesTruthAssignment(f.truthAssignment[..]);
+    }
+
+  method start_precondition_test()
+    // specification of input
+    requires formula.variablesCount == 2
+    requires formula.clauses == [[1]]
+    requires formula.clausesCount == 1
+    requires formula.clauseLength.Length == 1
+    requires formula.clauseLength[0] == 1
+    requires formula.truthAssignment.Length == 2
+    requires formula.truthAssignment[0] == -1
+    requires formula.truthAssignment[1] == -1
+    requires formula.trueLiteralsCount.Length == 1
+    requires formula.trueLiteralsCount[0] == 0
+    requires formula.falseLiteralsCount.Length == 1
+    requires formula.falseLiteralsCount[0] == 0
+    requires formula.positiveLiteralsToClauses.Length == 2
+    requires formula.negativeLiteralsToClauses.Length == 2
+    requires formula.positiveLiteralsToClauses[0] == [0]
+    requires formula.positiveLiteralsToClauses[1] == []
+    requires formula.negativeLiteralsToClauses[0] == []
+    requires formula.negativeLiteralsToClauses[1] == []
+    requires formula.decisionLevel == -1
+    requires formula.traceVariable.Length == 2
+    requires formula.traceVariable[0] == formula.traceVariable[1] == 0
+    requires formula.traceValue.Length == 2
+    requires formula.traceValue[0] == formula.traceValue[1] == false
+    requires formula.traceDLStart.Length == 2
+    requires formula.traceDLStart[0] == formula.traceDLStart[1] == 0
+    requires formula.traceDLEnd.Length == 2
+    requires formula.traceDLEnd[0] == formula.traceDLEnd[1] == 0
+    requires formula.assignmentsTrace == {}
+    // references
+    requires (formula.truthAssignment != formula.trueLiteralsCount) &&
+    (formula.truthAssignment != formula.falseLiteralsCount) &&
+    (formula.truthAssignment != formula.clauseLength) &&
+    (formula.truthAssignment != formula.traceVariable) &&
+    (formula.truthAssignment != formula.traceDLStart) &&
+    (formula.truthAssignment != formula.traceDLEnd) &&
+    (formula.trueLiteralsCount != formula.falseLiteralsCount) &&
+    (formula.trueLiteralsCount != formula.clauseLength) &&
+    (formula.trueLiteralsCount != formula.traceVariable) &&
+    (formula.trueLiteralsCount != formula.traceDLStart) &&
+    (formula.trueLiteralsCount != formula.traceDLEnd) &&
+    (formula.falseLiteralsCount != formula.clauseLength) &&
+    (formula.falseLiteralsCount != formula.traceVariable) &&
+    (formula.falseLiteralsCount != formula.traceDLStart) &&
+    (formula.falseLiteralsCount != formula.traceDLEnd) &&
+    (formula.clauseLength != formula.traceVariable) &&
+    (formula.clauseLength != formula.traceDLStart) &&
+    (formula.clauseLength != formula.traceDLEnd) &&
+    (formula.positiveLiteralsToClauses != formula.negativeLiteralsToClauses) &&
+    (formula.traceVariable != formula.traceDLStart) &&
+    (formula.traceVariable != formula.traceDLEnd) &&
+    (formula.traceDLStart != formula.traceDLEnd)
+    ensures old(formula.valid())
+    ensures old(formula.decisionLevel) == -1
+  {}
+
+
+  method start_counterexample() returns (result : SAT_UNSAT) // tau may be arbitrary truth assignment
+ // original specification
+    requires formula.valid();
+    requires formula.decisionLevel == -1;
+    modifies formula.truthAssignment, formula.traceVariable, formula.traceValue,
+              formula.traceDLStart, formula.traceDLEnd, formula`decisionLevel,
+              formula`assignmentsTrace, formula.trueLiteralsCount,
+              formula.falseLiteralsCount;
+      ensures formula.valid();
+    ensures result.SAT? ==> formula.validValuesTruthAssignment(result.tau);
+    ensures result.SAT? ==> formula.isSatisfiableExtend(old(formula.truthAssignment[..]));
+    ensures result.UNSAT? ==>
+      !formula.isSatisfiableExtend(old(formula.truthAssignment[..]));
+    // counterexample specific - a wrong behavior
+    ensures result.SAT? ==> result.tau[0] == -1
+  {
+  // original start() implementation:
     formula.level0UnitPropagation();
     result := solve();
+  // added at the end of original start() implementation:
+    if result.SAT? {
+      result := SAT(seq(formula.variablesCount, _ => -1));
+    } 
   }
 }
