truesat_src/solver/formula.dfy
@@ -9,15 +9,14 @@ class Formula extends DataStructures {
     clauses : seq<seq<Int32.t>>
   )
     requires InputPredicate.valid((variablesCount, clauses));
-
     ensures valid();
-
+    ensures this.variablesCount == variablesCount
+    ensures this.clauses == clauses
     ensures fresh(this.traceVariable) && fresh(this.traceValue) &&
       fresh(this.traceDLStart) && fresh(this.traceDLEnd) &&
       fresh(this.clauseLength) && fresh(this.trueLiteralsCount) &&
       fresh(this.falseLiteralsCount) && fresh(this.positiveLiteralsToClauses) &&
       fresh(this.negativeLiteralsToClauses) && fresh(this.truthAssignment);
-
     ensures this.decisionLevel == -1;
   {
     assert 0 < variablesCount < Int32.max;
@@ -30,23 +29,23 @@ class Formula extends DataStructures {
     this.clauses := clauses;
     this.decisionLevel := -1;
 
-    this.traceVariable := new Int32.t[variablesCount];
-    this.traceValue := new bool[variablesCount];
-    this.traceDLStart := new Int32.t[variablesCount];
-    this.traceDLEnd := new Int32.t[variablesCount];
+    this.traceVariable := new Int32.t[variablesCount](_=>0);
+    this.traceValue := new bool[variablesCount](_=>false);
+    this.traceDLStart := new Int32.t[variablesCount](_=>0);
+    this.traceDLEnd := new Int32.t[variablesCount](_=>0);
     this.assignmentsTrace := {};
 
     var clsLength := |clauses| as Int32.t;
     this.clausesCount := clsLength;
-    this.clauseLength := new Int32.t[clsLength];
+    this.clauseLength := new Int32.t[clsLength](_=>0);
 
-    this.trueLiteralsCount := new Int32.t[clsLength];
-    this.falseLiteralsCount := new Int32.t[clsLength];
+    this.trueLiteralsCount := new Int32.t[clsLength](_=>0);
+    this.falseLiteralsCount := new Int32.t[clsLength](_=>0);
 
-    this.positiveLiteralsToClauses := new seq<Int32.t>[variablesCount];
-    this.negativeLiteralsToClauses := new seq<Int32.t>[variablesCount];
+    this.positiveLiteralsToClauses := new seq<Int32.t>[variablesCount](_=>[]);
+    this.negativeLiteralsToClauses := new seq<Int32.t>[variablesCount](_=>[]);
 
-    this.truthAssignment := new Int32.t[variablesCount];
+    this.truthAssignment := new Int32.t[variablesCount](_=>0);
 
     new;
 
@@ -84,6 +83,11 @@ class Formula extends DataStructures {
     assert clauses == clauses[..clausesCount];
     assert countLiterals(clausesCount) == InputPredicate.countLiterals(clauses);
   }
+
+  lemma constructFormula(variablesCount : Int32.t,
+    clauses : seq<seq<Int32.t>>) returns (f:Formula)
+    
+
 
   lemma inputPredicate_countLiterals(cI : Int32.t)
     requires validVariablesCount();
@@ -1632,6 +1636,7 @@ class Formula extends DataStructures {
     requires isEmpty();
 
     ensures isSatisfiableExtend(truthAssignment[..]);
+    ensures isSatisfiableTruthAssignment(truthAssignment[..], truthAssignment[..])
   {
     assert forall i :: 0 <= i < |clauses| ==>
         trueLiteralsCount[i] > 0;
